AP/System/Invariant.lean
@@ -15,9 +15,9 @@ theorem invariant {p : S → Prop} {a b}
   exact h₃ h₁ h₂
 
 theorem invariant_init {p : S → Prop} {a}
-(h₁ : sys.Valid a) (h₂ : ∀ {a}, sys.Initial a → p a)
+(h₁ : sys.WF a) (h₂ : ∀ {a}, sys.Initial a → p a)
 (h₃ : ∀ {x y t}, p x → sys.trTo x t y → p y) : p a := by
-  rw [valid_iff] at h₁
+  rw [wf_iff] at h₁
   obtain ⟨s₀, h₁, h₄⟩ := h₁
   exact invariant (h₂ h₁) h₄ h₃
 
